proofs/lean/SpecRest/Translate.lean
@@ -25,6 +25,10 @@ def translate : Expr → SmtTerm
   | .boolBin .iff     l r =>
       .and (.implies (translate l) (translate r))
            (.implies (translate r) (translate l))
+  | .arith .add l r => .add (translate l) (translate r)
+  | .arith .sub l r => .sub (translate l) (translate r)
+  | .arith .mul l r => .mul (translate l) (translate r)
+  | .arith .div l r => .div (translate l) (translate r)
   | .cmp .eq  l r => .eq (translate l) (translate r)
   | .cmp .neq l r => .not (.eq (translate l) (translate r))
   | .cmp .lt  l r => .lt (translate l) (translate r)
